src/refinement/SimCertify.v
@@ -29,42 +29,35 @@ Inductive sim_time (ts:Time.t) (v1 v2:Time.t): Prop :=
 .
 Hint Constructors sim_time.
 
-Inductive sim_view (ts:Time.t) (forbid:Taint.t) (v1 v2:View.t (A:=Taint.t)): Prop :=
+Inductive sim_view (ts:Time.t) (v1 v2:View.t (A:=Taint.t)): Prop :=
 | sim_view_intro
-    (TS: v2.(View.ts) <= ts ->
-         v1 = v2 /\
-         v2.(View.annot) ∩₁ forbid ⊆₁ bot)
+    (TS: v2.(View.ts) <= ts -> v1 = v2)
 .
 Hint Constructors sim_view.
 
-Inductive sim_low_view (ts:Time.t) (forbid:Taint.t) (v1 v2:View.t (A:=Taint.t)): Prop :=
+Inductive sim_low_view (ts:Time.t) (v1 v2:View.t (A:=Taint.t)): Prop :=
 | sim_low_view_intro
     (TS: v2.(View.ts) <= ts)
     (VAL: v1 = v2)
-    (FORBID: v2.(View.annot) ∩₁ forbid ⊆₁ bot)
 .
 Hint Constructors sim_low_view.
 
-Inductive sim_val (ts:Time.t) (forbid:Taint.t) (v1 v2:ValA.t (A:=View.t (A:=Taint.t))): Prop :=
+Inductive sim_val (ts:Time.t) (v1 v2:ValA.t (A:=View.t (A:=Taint.t))): Prop :=
 | sim_val_intro
-    (TS: v2.(ValA.annot).(View.ts) <= ts ->
-         v1 = v2 /\
-         v2.(ValA.annot).(View.annot) ∩₁ forbid ⊆₁ bot)
+    (TS: v2.(ValA.annot).(View.ts) <= ts -> v1 = v2)
 .
 Hint Constructors sim_val.
 
-Inductive sim_rmap (ts:Time.t) (forbid:Taint.t) (rmap1 rmap2:RMap.t (A:=View.t (A:=Taint.t))): Prop :=
+Inductive sim_rmap (ts:Time.t) (rmap1 rmap2:RMap.t (A:=View.t (A:=Taint.t))): Prop :=
 | sim_rmap_intro
-    (RMAP: IdMap.Forall2
-             (fun _ => (sim_val ts forbid))
-             rmap1 rmap2)
+    (RMAP: IdMap.Forall2 (fun _ => sim_val ts) rmap1 rmap2)
 .
 Hint Constructors sim_rmap.
 
-Inductive sim_state (ts:Time.t) (forbid:Taint.t) (st1 st2:State.t (A:=View.t (A:=Taint.t))): Prop :=
+Inductive sim_state (ts:Time.t) (st1 st2:State.t (A:=View.t (A:=Taint.t))): Prop :=
 | sim_state_intro
     (STMTS: st1.(State.stmts) = st2.(State.stmts))
-    (RMAP: sim_rmap ts forbid st1.(State.rmap) st2.(State.rmap))
+    (RMAP: sim_rmap ts st1.(State.rmap) st2.(State.rmap))
 .
 Hint Constructors sim_state.
 
@@ -75,21 +68,21 @@ Inductive sim_exbank (tid:Id.t) (mem1 mem2:Memory.t) (ts1 ts2:Time.t): Prop :=
         Memory.exclusive tid loc ts1 (length mem1) mem1)
 .
 
-Inductive sim_lc (tid:Id.t) (ts:Time.t) (forbid:Taint.t) (lc1 lc2:Local.t (A:=Taint.t)) (mem1 mem2:Memory.t): Prop :=
+Inductive sim_lc (tid:Id.t) (ts:Time.t) (lc1 lc2:Local.t (A:=Taint.t)) (mem1 mem2:Memory.t): Prop :=
 | sim_lc_intro
     (COH: forall loc, sim_time ts (lc1.(Local.coh) loc) (lc2.(Local.coh) loc))
-    (VRP: sim_low_view ts forbid lc1.(Local.vrp) lc2.(Local.vrp))
-    (VWP: sim_low_view ts forbid lc1.(Local.vwp) lc2.(Local.vwp))
-    (VRM: sim_view ts forbid lc1.(Local.vrm) lc2.(Local.vrm))
-    (VWM: sim_view ts forbid lc1.(Local.vwm) lc2.(Local.vwm))
-    (VCAP: sim_low_view ts forbid lc1.(Local.vcap) lc2.(Local.vcap))
-    (VREL: sim_low_view ts forbid lc1.(Local.vrel) lc2.(Local.vrel))
+    (VRP: sim_low_view ts lc1.(Local.vrp) lc2.(Local.vrp))
+    (VWP: sim_low_view ts lc1.(Local.vwp) lc2.(Local.vwp))
+    (VRM: sim_view ts lc1.(Local.vrm) lc2.(Local.vrm))
+    (VWM: sim_view ts lc1.(Local.vwm) lc2.(Local.vwm))
+    (VCAP: sim_low_view ts lc1.(Local.vcap) lc2.(Local.vcap))
+    (VREL: sim_low_view ts lc1.(Local.vrel) lc2.(Local.vrel))
     (FWDBANK: forall loc,
         opt_rel
           (fun fwd1 fwd2 =>
              fwd2.(FwdItem.ts) <= ts ->
              (fwd1.(FwdItem.ts) = fwd2.(FwdItem.ts) /\
-              sim_low_view ts forbid fwd1.(FwdItem.view) fwd2.(FwdItem.view) /\
+              sim_low_view ts fwd1.(FwdItem.view) fwd2.(FwdItem.view) /\
               fwd1.(FwdItem.ex) = fwd2.(FwdItem.ex)))
           (lc1.(Local.fwdbank) loc) (lc2.(Local.fwdbank) loc))
     (EXBANK: opt_rel (sim_exbank tid mem1 mem2) lc1.(Local.exbank) lc2.(Local.exbank))
@@ -98,7 +91,7 @@ Inductive sim_lc (tid:Id.t) (ts:Time.t) (forbid:Taint.t) (lc1 lc2:Local.t (A:=Ta
 .
 Hint Constructors sim_lc.
 
-Inductive sim_mem (tid:Id.t) (ts:Time.t) (forbid:Taint.t) (mem1 mem2:Memory.t): Prop :=
+Inductive sim_mem (tid:Id.t) (ts:Time.t) (mem1 mem2:Memory.t): Prop :=
 | sim_mem_intro
     mem_prefix mem1' mem2' msg
     (LEN: ts = length mem_prefix)
@@ -107,45 +100,43 @@ Inductive sim_mem (tid:Id.t) (ts:Time.t) (forbid:Taint.t) (mem1 mem2:Memory.t): 
     (TID: List.Forall (fun msg => msg.(Msg.tid) = tid) mem1')
     (TID: List.Forall (fun msg => msg.(Msg.tid) = tid) mem2')
     (MSG: msg.(Msg.tid) <> tid)
-    (FORBID: forbid = (fun taint => exists id, taint = Taint.R id 0))
 .
 Hint Constructors sim_mem.
 
-Inductive sim_eu (tid:Id.t) (ts:Time.t) (forbid:Taint.t) (eu1 eu2:ExecUnit.t (A:=Taint.t)): Prop :=
+Inductive sim_eu (tid:Id.t) (ts:Time.t) (eu1 eu2:ExecUnit.t (A:=Taint.t)): Prop :=
 | sim_eu_intro
-    (STATE: sim_state ts forbid eu1.(ExecUnit.state) eu2.(ExecUnit.state))
-    (LOCAL: sim_lc tid ts forbid eu1.(ExecUnit.local) eu2.(ExecUnit.local) eu1.(ExecUnit.mem) eu2.(ExecUnit.mem))
-    (MEM: sim_mem tid ts forbid eu1.(ExecUnit.mem) eu2.(ExecUnit.mem))
+    (STATE: sim_state ts eu1.(ExecUnit.state) eu2.(ExecUnit.state))
+    (LOCAL: sim_lc tid ts eu1.(ExecUnit.local) eu2.(ExecUnit.local) eu1.(ExecUnit.mem) eu2.(ExecUnit.mem))
+    (MEM: sim_mem tid ts eu1.(ExecUnit.mem) eu2.(ExecUnit.mem))
 .
 Hint Constructors sim_eu.
 
-Inductive sim_aeu (tid:Id.t) (ts:Time.t) (forbid:Taint.t) (aeu1 aeu2:AExecUnit.t): Prop :=
+Inductive sim_aeu (tid:Id.t) (ts:Time.t) (aeu1 aeu2:AExecUnit.t): Prop :=
 | sim_aeu_intro
-    (EU: sim_eu tid ts forbid aeu1.(AExecUnit.eu) aeu2.(AExecUnit.eu))
+    (EU: sim_eu tid ts aeu1.(AExecUnit.eu) aeu2.(AExecUnit.eu))
     (AUX: aeu1.(AExecUnit.aux) = aeu2.(AExecUnit.aux))
-    (AUX_FORBID: aeu2.(AExecUnit.aux).(AExecUnit.taint) ∩₁ forbid ⊆₁ bot)
 .
 Hint Constructors sim_aeu.
 
-Inductive sim_event ts forbid: forall (e1 e2:Event.t (A:=View.t (A:=Taint.t))), Prop :=
+Inductive sim_event ts: forall (e1 e2:Event.t (A:=View.t (A:=Taint.t))), Prop :=
 | sim_event_internal
     ctrl1 ctrl2
-    (CTRL: sim_view ts forbid ctrl1 ctrl2):
-    sim_event ts forbid (Event.internal ctrl1) (Event.internal ctrl2)
+    (CTRL: sim_view ts ctrl1 ctrl2):
+    sim_event ts (Event.internal ctrl1) (Event.internal ctrl2)
 | sim_event_read
     ex ord vloc1 vloc2 res1 res2
-    (VLOC: sim_val ts forbid vloc1 vloc2)
-    (RES: sim_val ts forbid res1 res2):
-    sim_event ts forbid (Event.read ex ord vloc1 res1) (Event.read ex ord vloc2 res2)
+    (VLOC: sim_val ts vloc1 vloc2)
+    (RES: sim_val ts res1 res2):
+    sim_event ts (Event.read ex ord vloc1 res1) (Event.read ex ord vloc2 res2)
 | sim_event_write
     ex ord vloc1 vloc2 vval1 vval2 res1 res2
-    (VLOC: sim_val ts forbid vloc1 vloc2)
-    (VVAL: sim_val ts forbid vval1 vval2)
-    (RES: sim_val ts forbid res1 res2):
-    sim_event ts forbid (Event.write ex ord vloc1 vval1 res1) (Event.write ex ord vloc2 vval2 res2)
+    (VLOC: sim_val ts vloc1 vloc2)
+    (VVAL: sim_val ts vval1 vval2)
+    (RES: sim_val ts res1 res2):
+    sim_event ts (Event.write ex ord vloc1 vval1 res1) (Event.write ex ord vloc2 vval2 res2)
 | sim_event_barrier
     b:
-    sim_event ts forbid (Event.barrier b) (Event.barrier b)
+    sim_event ts (Event.barrier b) (Event.barrier b)
 .
 
 Lemma sim_time_join
@@ -160,31 +151,31 @@ Proof.
 Qed.
 
 Lemma sim_val_const
-      ts forbid c:
-  sim_val ts forbid (ValA.mk _ c bot) (ValA.mk _ c bot).
+      ts c:
+  sim_val ts (ValA.mk _ c bot) (ValA.mk _ c bot).
 Proof.
-  econs. s. i. splits; ss. ii. inv H0. ss.
+  econs. ss.
 Qed.
 
 Lemma sim_view_bot
-      ts forbid:
-  sim_view ts forbid bot bot.
+      ts:
+  sim_view ts bot bot.
 Proof.
-  econs. i. splits; ss. ii. inv H0. ss.
+  econs. ss.
 Qed.
 
 Lemma sim_view_const
-      ts forbid c:
-  sim_view ts forbid (View.mk c bot) (View.mk c bot).
+      ts c:
+  sim_view ts (View.mk c bot) (View.mk c bot).
 Proof.
-  econs. i. splits; ss. ii. inv H0. ss.
+  econs. ss.
 Qed.
 
 Lemma sim_view_join
-      ts forbid l1 l2 r1 r2
-      (VIEW1: sim_view ts forbid l1 r1)
-      (VIEW2: sim_view ts forbid l2 r2):
-  sim_view ts forbid (join l1 l2) (join r1 r2).
+      ts l1 l2 r1 r2
+      (VIEW1: sim_view ts l1 r1)
+      (VIEW2: sim_view ts l2 r2):
+  sim_view ts (join l1 l2) (join r1 r2).
 Proof.
   destruct l1 as [lt1 lv1].
   destruct l2 as [lt2 lv2].
@@ -192,99 +183,85 @@ Proof.
   destruct r2 as [rt2 rv2].
   inv VIEW1. inv VIEW2. ss.
   econs. s. intro X. unfold join, Time.join in X. apply Time.max_lub_iff in X. des.
-  specialize (TS X). specialize (TS0 X0). des. inv TS. inv TS0.
-  splits; ss. ii. inv H. inv H0.
-  - apply TS2. ss.
-  - apply TS1. ss.
+  specialize (TS X). specialize (TS0 X0). des. inv TS. inv TS0. ss.
 Qed.
 
 Lemma sim_view_low_view
-      ts forbid l r
-      (VIEW: sim_view ts forbid l r)
+      ts l r
+      (VIEW: sim_view ts l r)
       (TS: r.(View.ts) <= ts):
-  sim_low_view ts forbid l r.
+  sim_low_view ts l r.
 Proof.
   inv VIEW. specialize (TS0 TS). des. econs; ss.
 Qed.
 
 Lemma sim_low_view_bot
-      ts forbid:
-  sim_low_view ts forbid bot bot.
+      ts:
+  sim_low_view ts bot bot.
 Proof.
-  econs; ss.
-  - apply bot_spec.
-  - ii. inv H. ss.
+  econs; ss. apply bot_spec.
 Qed.
 
 Lemma sim_low_view_const
-      ts forbid c
+      ts c
       (TS: c <= ts):
-  sim_low_view ts forbid (View.mk c bot) (View.mk c bot).
+  sim_low_view ts (View.mk c bot) (View.mk c bot).
 Proof.
-  econs; ss. ii. inv H. ss.
+  econs; ss.
 Qed.
 
 Lemma sim_low_view_join
-      ts forbid l1 l2 r1 r2
-      (VIEW1: sim_low_view ts forbid l1 r1)
-      (VIEW2: sim_low_view ts forbid l2 r2):
-  sim_low_view ts forbid (join l1 l2) (join r1 r2).
+      ts l1 l2 r1 r2
+      (VIEW1: sim_low_view ts l1 r1)
+      (VIEW2: sim_low_view ts l2 r2):
+  sim_low_view ts (join l1 l2) (join r1 r2).
 Proof.
   destruct l1 as [lt1 lv1].
   destruct l2 as [lt2 lv2].
   destruct r1 as [rt1 rv1].
   destruct r2 as [rt2 rv2].
   inv VIEW1. inv VIEW2. ss. inv VAL. inv VAL0.
-  econs; ss.
-  - apply join_spec; ss.
-  - ii. inv H. inv H0.
-    + apply FORBID. ss.
-    + apply FORBID0. ss.
+  econs; ss. apply join_spec; ss.
 Qed.
 
-Lemma sim_val_view ts forbid v1 v2
-      (VAL: sim_val ts forbid v1 v2):
-  sim_view ts forbid v1.(ValA.annot) v2.(ValA.annot).
+Lemma sim_val_view ts v1 v2
+      (VAL: sim_val ts v1 v2):
+  sim_view ts v1.(ValA.annot) v2.(ValA.annot).
 Proof.
   inv VAL. econs. i. specialize (TS H). des. subst. ss.
 Qed.
 
 Lemma sim_rmap_expr
-      ts forbid rmap1 rmap2 e
-      (RMAP: sim_rmap ts forbid rmap1 rmap2):
-  sim_val ts forbid (sem_expr rmap1 e) (sem_expr rmap2 e).
+      ts rmap1 rmap2 e
+      (RMAP: sim_rmap ts rmap1 rmap2):
+  sim_val ts (sem_expr rmap1 e) (sem_expr rmap2 e).
 Proof.
   induction e; s.
   - apply sim_val_const.
   - unfold RMap.find. inv RMAP. specialize (RMAP0 reg). inv RMAP0; ss.
-    apply sim_val_const.
-  - econs. s. i. inv IHe. specialize (TS H). des. splits; ss. congr.
+  - econs. s. i. inv IHe. specialize (TS H). des. congr.
   - econs. s. i. unfold join, Time.join in H. apply Time.max_lub_iff in H. des.
     inv IHe1. inv IHe2.
-    specialize (TS H). specialize (TS0 H0). des. splits; ss.
-    + congr.
-    + ii. inv H1. inv H2.
-      * apply TS2. ss.
-      * apply TS1. ss.
+    specialize (TS H). specialize (TS0 H0). des. congr.
 Qed.
 
 Lemma sim_rmap_add
-      ts forbid rmap1 rmap2 v1 v2 r
-      (RMAP: sim_rmap ts forbid rmap1 rmap2)
-      (VAL: sim_val ts forbid v1 v2):
-  sim_rmap ts forbid (RMap.add r v1 rmap1) (RMap.add r v2 rmap2).
+      ts rmap1 rmap2 v1 v2 r
+      (RMAP: sim_rmap ts rmap1 rmap2)
+      (VAL: sim_val ts v1 v2):
+  sim_rmap ts (RMap.add r v1 rmap1) (RMap.add r v2 rmap2).
 Proof.
   inv RMAP. econs. ii. unfold RMap.add. rewrite ? IdMap.add_spec.
   condtac; ss. inversion e. subst. econs. ss.
 Qed.
 
 Lemma sim_aeu_step
-      tid ts forbid aeu1 aeu2 aeu2'
-      (SIM: sim_aeu tid ts forbid aeu1 aeu2)
+      tid ts aeu1 aeu2 aeu2'
+      (SIM: sim_aeu tid ts aeu1 aeu2)
       (STEP: AExecUnit.step tid aeu2 aeu2'):
   exists aeu1',
     <<STEP: AExecUnit.step tid aeu1 aeu1'>> /\
-    <<SIM: sim_aeu tid ts forbid aeu1' aeu2'>>.
+    <<SIM: sim_aeu tid ts aeu1' aeu2'>>.
 Proof.
   destruct aeu1 as [[[stmts1 rmap1] lc1 mem1] aux1].
   destruct aeu2 as [[[stmts2 rmap2] lc2 mem2] aux2].
@@ -302,7 +279,8 @@ Proof.
       + left. econs; ss. econs; ss; cycle 1.
         * econs 1; eauto. econs; eauto.
         * s. econs 1.
-      + econs; ss. econs; ss. inv LOCAL0. econs; ss.
+      + econs; ss. econs; ss.
+        inv LOCAL0. econs; ss.
         apply sim_low_view_join; ss. apply sim_low_view_bot.
     - (* assign *)
       inv LC.
@@ -354,9 +332,7 @@ Proof.
               admit. (* memory no_msgs *)
             * admit. (* memory read *)
           + econs 3; ss.
-        - econs; ss; cycle 1.
-          { destruct ex; ss. }
-          econs; ss.
+        - econs; ss. econs; ss.
           + admit. (* sim_state *)
           + admit. (* sim_lc *)
       }
@@ -371,10 +347,8 @@ Proof.
       + left. econs; ss. econs; ss; cycle 1.
         * econs 4; eauto. econs; eauto.
         * s. econs 4; ss.
-      + econs; ss; cycle 1.
-        * ii. apply AUX_FORBID. inv H. econs; ss. inv H0; ss.
-        * econs; ss; eauto using sim_rmap_add, sim_val_const.
-          inv LOCAL0. econs; ss.
+      + econs; ss. econs; ss; eauto using sim_rmap_add, sim_val_const.
+        inv LOCAL0. econs; ss.
     - (* isb *)
       inv STEP.
       eexists (AExecUnit.mk (ExecUnit.mk _ _ _) _). esplits.
@@ -420,12 +394,12 @@ Proof.
 Admitted.
 
 Lemma sim_aeu_rtc_step
-      tid ts forbid aeu1 aeu2 aeu2'
-      (SIM: sim_aeu tid ts forbid aeu1 aeu2)
+      tid ts aeu1 aeu2 aeu2'
+      (SIM: sim_aeu tid ts aeu1 aeu2)
       (STEP: rtc (AExecUnit.step tid) aeu2 aeu2'):
   exists aeu1',
     <<STEP: rtc (AExecUnit.step tid) aeu1 aeu1'>> /\
-    <<SIM: sim_aeu tid ts forbid aeu1' aeu2'>>.
+    <<SIM: sim_aeu tid ts aeu1' aeu2'>>.
 Proof.
   revert aeu1 SIM. induction STEP.
   { i. esplits; eauto. }
@@ -434,7 +408,156 @@ Proof.
   esplits; [|by eauto]. econs; eauto.
 Qed.
 
-Lemma certify_lift_diff
+Lemma lift_wf
+      tid (eu1 eu2:ExecUnit.t (A:=unit)) msg
+      (WF: ExecUnit.wf tid eu1)
+      (ST: eu2.(ExecUnit.state) = eu1.(ExecUnit.state))
+      (LC: eu2.(ExecUnit.local) = eu1.(ExecUnit.local))
+      (MEM: eu2.(ExecUnit.mem) = eu1.(ExecUnit.mem) ++ [msg])
+      (MSG: msg.(Msg.tid) <> tid):
+  ExecUnit.wf tid eu2.
+Proof.
+  destruct eu1 as [st1 lc1 mem1].
+  destruct eu2 as [st2 lc2 mem2].
+  ss. subst. inv WF. ss. econs; ss.
+  - apply ExecUnit.rmap_append_wf. ss.
+  - inv LOCAL. econs; try rewrite app_length; intuition.
+    + exploit FWDBANK; eauto. i. des. intuition.
+    + exploit FWDBANK; eauto. i. des. intuition.
+    + apply Memory.get_msg_snoc_inv in MSG0. des; eauto.
+      subst. ss.
+Qed.
+
+Inductive sound_taint (loc:Loc.t) (v:Taint.t): Prop :=
+| sound_taint_intro
+    (TAINT: forall from to, ~ v (Taint.W from to loc))
+.
+
+Inductive sound_view (loc:Loc.t) (v:View.t (A:=Taint.t)): Prop :=
+| sound_view_intro
+    (VIEW: sound_taint loc v.(View.annot))
+.
+
+Inductive sound_val (loc:Loc.t) (v:ValA.t (A:=View.t (A:=Taint.t))): Prop :=
+| sound_val_intro
+    (VAL: sound_view loc v.(ValA.annot))
+.
+
+Inductive sound_st (loc:Loc.t) (st:State.t (A:=View.t (A:=Taint.t))): Prop :=
+| sound_st_intro
+    (RMAP: IdMap.Forall (fun _ => sound_val loc) st.(State.rmap))
+.
+
+Inductive sound_lc (is_first_ex:bool) (ts:Time.t) (loc:Loc.t) (lc:Local.t (A:=Taint.t)): Prop :=
+| sound_lc_intro
+    (VRP: sound_view loc lc.(Local.vrp))
+    (VWP: sound_view loc lc.(Local.vwp))
+    (VRM: sound_view loc lc.(Local.vrm))
+    (VWM: sound_view loc lc.(Local.vwm))
+    (VCAP: sound_view loc lc.(Local.vcap))
+    (VREL: sound_view loc lc.(Local.vrel))
+    (FWDBANK: forall l fwd (FWD: lc.(Local.fwdbank) l = Some fwd), sound_view loc fwd.(FwdItem.view))
+    (EXBANK: is_first_ex -> forall exbank (EXBANK: lc.(Local.exbank) = Some exbank), exbank <= ts)
+.
+
+Inductive sound_aeu (loc:Loc.t) (ts:Time.t) (aeu:AExecUnit.t): Prop :=
+| sound_aeu_intro
+    (ST: sound_st loc aeu.(ExecUnit.state))
+    (LC: sound_lc (aeu.(AExecUnit.aux).(AExecUnit.ex_counter) == 0) ts loc aeu.(ExecUnit.local))
+    (AUX: sound_taint loc aeu.(AExecUnit.aux).(AExecUnit.taint))
+.
+
+Lemma sound_aeu_step
+      loc ts tid aeu1 aeu2
+      (STEP: AExecUnit.step tid aeu1 aeu2)
+      (SOUND: sound_aeu loc ts aeu1):
+  sound_aeu loc ts aeu2.
+Proof.
+  destruct aeu1 as [[st1 lc1 mem1] aux1].
+  destruct aeu2 as [[st2 lc2 mem2] aux2].
+  inv SOUND. ss. inv STEP.
+  { inv STEP0. inv STEP. ss. subst.
+    inv ST. inv LC.
+    inv LOCAL; inv STATE; ss. 
+    - inv LC. econs; ss. econs; ss.
+      admit. (* soudn view bot join *)
+    - inv LC. econs; ss.
+      + admit. (* sound rmap addd expr *)
+      + econs; ss. admit. (* soudn view bot join *)
+    - inv LC. econs; ss.
+      econs; ss. admit. (* sound join expr *)
+    - inv LC. econs; ss.
+      econs; ss. admit. (* sound join bot *)
+    - inv STEP. econs; ss.
+      + econs; ss. admit.
+      + admit.
+      + destruct ex; ss.
+    - inv STEP. econs; ss.
+      + econs; ss. admit.
+      + admit.
+      + admit.
+    - inv STEP. econs; ss.
+      + econs; ss. admit.
+      + admit.
+    - inv STEP. econs; ss.
+      econs; ss. admit.
+    - inv STEP. econs; ss.
+      econs; ss. admit.
+    - inv STEP. econs; ss.
+      econs; ss.
+      admit.
+      admit.
+    - inv STEP. econs; ss.
+      econs; ss.
+      admit.
+      admit.
+  }
+  { inv STEP0. ss. subst.
+    inv ST. inv LC.
+    inv LOCAL. inv STATE. econs; ss.
+    - econs; ss. admit.
+    - econs; ss.
+      all: admit.
+  }
+Admitted.
+
+Lemma sound_rtc_aeu_step
+      loc ts tid aeu1 aeu2
+      (STEP: rtc (AExecUnit.step tid) aeu1 aeu2)
+      (SOUND: sound_aeu loc ts aeu1):
+  sound_aeu loc ts aeu2.
+Proof.
+  revert SOUND. induction STEP; ss. i. exploit sound_aeu_step; eauto.
+Qed.
+
+Lemma certify_diff_not_locked
+      tid (eu:ExecUnit.t (A:=unit)) lock mem msg
+      (CERTIFY: certify tid eu lock)
+      (WF: ExecUnit.wf tid eu)
+      (MEM: eu.(ExecUnit.mem) = mem ++ [msg])
+      (MSG: msg.(Msg.tid) <> tid):
+  ~ Lock.is_locked lock bot msg.(Msg.loc).
+Proof.
+  inv CERTIFY.
+  exploit sound_rtc_aeu_step; eauto.
+  { instantiate (1 := (length mem)).
+    instantiate (1 := msg.(Msg.loc)).
+    destruct eu as [st1 lc1 mem1]. ss. subst.
+    econs.
+    - econs. s. ii. revert FIND.
+      unfold AExecUnit.init_rmap. rewrite IdMap.map_spec.
+      destruct (IdMap.find id (State.rmap st1)); ss. i. inv FIND.
+      econs. econs. econs. ss.
+    - s. admit.
+    - econs. ss.
+  }
+  ii. destruct lock as [ex release]. ss. subst.
+  inv H. destruct exlock as [from to loc]. ss. subst.
+  inv RANGE. inv H. inv LOCK. ss.
+  eapply x0. eauto.
+Admitted.
+
+Lemma lift_certify_diff
       tid (eu1 eu2:ExecUnit.t (A:=unit)) lock msg
       (CERTIFY: certify tid eu2 lock)
       (WF: ExecUnit.wf tid eu1)
@@ -445,43 +568,34 @@ Lemma certify_lift_diff
   <<CERTIFY: certify tid eu1 lock>> /\
   <<NOLOCK: ~ Lock.is_locked lock bot msg.(Msg.loc)>>.
 Proof.
+  exploit lift_wf; eauto. i.
+  splits; cycle 1.
+  { eapply certify_diff_not_locked; eauto. }
   destruct eu1 as [st1 lc1 mem1].
   destruct eu2 as [st2 lc2 mem2].
   ss. subst. inv CERTIFY.
   exploit sim_aeu_rtc_step; eauto.
-  { instantiate (1 := AExecUnit.init (ExecUnit.mk st1 lc1 mem1)). econs; ss.
-    - econs; ss; cycle 2.
-      + econs; ss. rewrite List.app_nil_r. ss.
-      + econs; ss. econs. ii.
-        unfold AExecUnit.init_rmap. rewrite IdMap.map_spec.
-        destruct (IdMap.find id (State.rmap st1)); ss. econs. econs; ss.
-        splits; ss. ii. inv H0. ss.
-      + unfold AExecUnit.init_lc, AExecUnit.init_view.
-        econs; ss; eauto using sim_view_const.
-        * admit. (* TODO: bug on init vcap *)
-        * admit. (* big vwp *)
-        * admit. (* big vcap *)
-        * admit. (* big vrel *)
-        * i. destruct (Local.fwdbank lc1 loc); ss. econs; ss.
-          splits; ss. apply sim_low_view_const.
-          admit. (* big fwd view *)
-        * destruct lc1. s. destruct exbank; ss. econs.
-          econs; eauto. ii. eapply H; eauto.
-          { apply Memory.read_mon. eauto. }
-          { rewrite app_length. lia. }
-          { exploit nth_error_Some. rewrite MSG0. intros [X _]. exploit X; ss. i.
-            rewrite nth_error_app1; ss.
-          }
-        * inv WF. inv LOCAL. ss.
-    - ii. inv H. inv H0.
+  { instantiate (1 := AExecUnit.init tid (ExecUnit.mk st1 lc1 mem1)). econs; ss.
+    econs; ss; cycle 2.
+    - econs; ss. rewrite List.app_nil_r. ss.
+    - econs; ss. econs. ii.
+      unfold AExecUnit.init_rmap. rewrite IdMap.map_spec.
+      destruct (IdMap.find id (State.rmap st1)); ss. econs. econs; ss.
+    - unfold AExecUnit.init_lc, AExecUnit.init_view.
+      inv WF. ss. inv LOCAL.
+      econs; ss; eauto using sim_view_const, sim_low_view_const.
+      + i. destruct (Local.fwdbank lc1 loc) eqn:FWD; ss. econs; ss.
+        splits; ss. apply sim_low_view_const. eapply FWDBANK. eauto.
+      + destruct lc1. s. destruct exbank; ss. econs.
+        econs; eauto. ii. eapply H; eauto.
+        * apply Memory.read_mon. eauto.
+        * rewrite app_length. lia.
+        * exploit nth_error_Some. rewrite MSG0. intros [X _]. exploit X; ss. i.
+          rewrite nth_error_app1; ss.
   }
-  i. des. esplits.
-  - econs; eauto.
-    + inv SIM. inv EU. inv LOCAL. etrans; eauto.
-    + inv SIM. congr.
-    + inv SIM. congr.
-  - intro X. inv X. destruct exlock as [loc from to]. ss. subst.
-    des. inv RANGE.
-    rewrite EX in LOCK. inv LOCK. ss.
-    inv SIM. eapply AUX_FORBID. econs; cycle 1; eauto.
-Admitted.
+  i. des.
+  econs; eauto.
+  - inv SIM. inv EU. inv LOCAL. etrans; eauto.
+  - inv SIM. congr.
+  - inv SIM. congr.
+Qed.
